Address review feedback

rocq-skylabs-brick/theories/lang/cpp/model/simple_pred.v
@@ -816,6 +816,13 @@ Module SimpleCPP.
     Instance type_ptr_affine σ p ty : Affine (type_ptr ty p) := _.
     Instance type_ptr_timeless σ p ty : Timeless (type_ptr ty p) := _.
 
+    Lemma type_ptr_drop_loc_info {resolve : genv} ty p :
+      type_ptr (resolve:=resolve) ty p -|- type_ptr (drop_loc_info ty) p.
+    Proof.
+      rewrite /type_ptr /aligned_ptr_ty align_of_drop_loc_info size_of_drop_loc_info.
+      rewrite /o_sub drop_loc_info_idemp. repeat f_equiv; apply proof_irrel.
+    Qed.
+
     Lemma type_ptr_off_nonnull {ty p o} :
       type_ptr ty (p ,, o) |-- [| p <> nullptr |].
     Admitted.
@@ -918,6 +925,7 @@ Module SimpleCPP.
     Qed.
 
     Definition tptsto (t : type) (q : cQp.t) (p : ptr) (v : val) : mpred :=
+      let t := drop_loc_info t in
       [| p <> nullptr |] ** [| is_heap_type t |] **
       Exists (oa : option addr),
         type_ptr t p ** (* use the appropriate ghost state instead *)
@@ -930,10 +938,15 @@ Module SimpleCPP.
     #[global] Instance tptsto_valid_type
       : forall (t : type) (q : cQp.t) (a : ptr) (v : val),
         Observe [| is_heap_type t |] (tptsto t q a v).
-    Proof. rewrite /tptsto; refine _. Qed.
+    Proof. intros; rewrite /tptsto /is_heap_type drop_loc_info_idemp; refine _. Qed.
+
+    Theorem tptsto_loc_info li ty q p v :
+      tptsto (TLocInfo li ty) q p v -|- tptsto ty q p v.
+    Proof. done. Qed.
 
     #[global] Instance tptsto_type_ptr : forall ty q p v,
-        Observe (type_ptr ty p) (tptsto ty q p v) := _.
+        Observe (type_ptr ty p) (tptsto ty q p v).
+    Proof. intros. rewrite type_ptr_drop_loc_info. apply _. Qed.
 
     (* TODO (JH): We shouldn't be axiomatizing this in our model in the long-run *)
     Axiom tptsto_live : forall ty (q : cQp.t) p v,
@@ -954,7 +967,12 @@ Module SimpleCPP.
       Timeless (tptsto ty q p v) := _.
 
     #[global] Instance tptsto_nonvoid ty (q : cQp.t) p v :
-      Observe [| ty <> Tvoid |] (tptsto ty q p v) := _.
+      Observe [| ty <> Tvoid |] (tptsto ty q p v).
+    Proof.
+      apply: observe_intro_persistent. iIntros "H".
+      iDestruct (observe [| drop_loc_info ty <> Tvoid |] with "H") as %Hty.
+      iPureIntro. by intros ->.
+    Qed.
 
     #[global] Instance tptsto_cfrac_valid ty :
       CFracValid2 (tptsto ty).
@@ -1142,7 +1160,7 @@ Module SimpleCPP.
       [| has_type_prop v ty |] **
       match v with
       | Vptr p =>
-        match drop_qualifiers ty with
+        match drop_loc_info (drop_qualifiers ty) with
         | Tptr ty =>
           valid_ptr p ** [| aligned_ptr_ty ty p |]
         | Tref ty | Trv_ref ty =>
@@ -1187,7 +1205,14 @@ Module SimpleCPP.
         destruct v => //.
         have H' : nonptr_prim_type (drop_qualifiers ty).
         { by rewrite -nonptr_prim_type_drop_qualifiers. }
-        destruct (drop_qualifiers ty); cbn in H' |- *; try contradiction; done.
+        destruct (drop_loc_info (drop_qualifiers ty)); cbn in H' |- *; try contradiction; done.
+      Qed.
+
+      Theorem has_type_loc_info li ty v :
+        has_type v (TLocInfo li ty) -|- has_type v ty.
+      Proof.
+        rewrite /has_type /= has_type_prop_loc_info.
+        destruct v; cbn; done.
       Qed.
 
       Lemma has_type_erase_qualifiers ty v :
@@ -1197,12 +1222,12 @@ Module SimpleCPP.
         f_equiv.
         rewrite -nonptr_prim_type_erase_qualifiers.
         case_match; eauto.
-        rewrite -erase_drop_qualifiers.
+        rewrite -erase_drop_qualifiers drop_loc_info_erase_qualifiers.
         case_match; simpl; eauto.
         all: try f_equiv.
         all: try rewrite aligned_ptr_ty_erase_qualifiers; auto.
         all: try apply stict_valid_if_not_empty_array_erase.
-        exfalso; by eapply unqual_drop_qualifiers.
+        exfalso; by eapply unqual_drop_loc_info_drop_qualifiers.
       Qed.
 
       Lemma has_type_nullptr' p :
