rocq-skylabs-brick/theories/lang/cpp/logic/wp.v
@@ -633,7 +633,7 @@ Section with_cpp.
   (* END wp_lval *)
 
   Axiom wp_lval_loc_info : forall {σ : genv} tu ρ li e Q,
-      wp_lval tu ρ (ELocInfo li e) Q = wp_lval tu ρ e Q.
+      wp_lval tu ρ (ELocInfo li e) Q -|- wp_lval tu ρ e Q.
 
   Axiom wp_lval_shift : forall {σ:genv} tu ρ e Q,
       (|={top}=> wp_lval tu ρ e (fun v free => |={top}=> Q v free))
@@ -803,11 +803,8 @@ Section with_cpp.
                         mpred. (* pre-condition *)
   (* END wp_init *)
 
-  Axiom wp_init_type_loc_info : forall {σ : genv} tu ρ li ty p e Q,
-      wp_init tu ρ (TLocInfo li ty) p e Q = wp_init tu ρ ty p e Q.
-
   Axiom wp_init_expr_loc_info : forall {σ : genv} tu ρ ty p li e Q,
-      wp_init tu ρ ty p (ELocInfo li e) Q = wp_init tu ρ ty p e Q.
+      wp_init tu ρ ty p (ELocInfo li e) Q -|- wp_init tu ρ ty p e Q.
 
   Axiom wp_init_shift : forall {σ:genv} tu ρ ty p e Q,
       (|={top}=> wp_init tu ρ ty p e (fun frees => |={top}=> Q frees))
@@ -831,6 +828,10 @@ Section with_cpp.
   *)
   Axiom wp_init_type_equiv : forall (σ : genv) tu ρ ty1 ty2 p e Q,
     ty1 ≡ ty2 -> wp_init tu ρ ty1 p e Q -|- wp_init tu ρ ty2 p e Q.
+
+  Lemma wp_init_type_loc_info : forall {σ : genv} tu ρ li ty p e Q,
+      wp_init tu ρ (TLocInfo li ty) p e Q -|- wp_init tu ρ ty p e Q.
+  Proof. intros. apply wp_init_type_equiv, TLocInfo_equiv. Qed.
 
   Section wp_init_proper.
     Context {σ : genv}.
@@ -916,7 +917,7 @@ Section with_cpp.
   (* END wp_operand *)
 
   Axiom wp_operand_loc_info : forall {σ : genv} tu ρ li e Q,
-      wp_operand tu ρ (ELocInfo li e) Q = wp_operand tu ρ e Q.
+      wp_operand tu ρ (ELocInfo li e) Q -|- wp_operand tu ρ e Q.
 
   Axiom wp_operand_shift : forall {σ:genv} tu ρ e Q,
       (|={top}=> wp_operand tu ρ e (fun v free => |={top}=> Q v free))
@@ -1032,7 +1033,7 @@ Section with_cpp.
     : forall {resolve:genv}, translation_unit -> region -> Expr -> M ptr.
 
   Axiom wp_xval_loc_info : forall {σ : genv} tu ρ li e Q,
-      wp_xval tu ρ (ELocInfo li e) Q = wp_xval tu ρ e Q.
+      wp_xval tu ρ (ELocInfo li e) Q -|- wp_xval tu ρ e Q.
 
   Axiom wp_xval_well_typed : forall {σ:genv} tu ρ e Q,
       wp_xval tu ρ e (fun v free => reference_to (type_of e) v -* Q v free)
@@ -1325,7 +1326,7 @@ Section with_cpp.
 
   (** An outer location wrapper has no effect on statement semantics. *)
   Axiom wp_loc_info : forall σ tu ρ li s Q,
-      wp (resolve:=σ) tu ρ (SLocInfo li s) Q = wp tu ρ s Q.
+      wp (resolve:=σ) tu ρ (SLocInfo li s) Q -|- wp tu ρ s Q.
 
   #[global] Declare Instance wp_ne : forall σ n,
     Proper (eq ==> eq ==> eq ==> dist n ==> dist n) (@wp σ).
