rocq-skylabs-brick/theories/lang/cpp/semantics/values.v
@@ -373,6 +373,9 @@ Module Type RAW_BYTES_MIXIN
   | Vqual t ty v1 v2 :
     val_related ty v1 v2 ->
     val_related (Tqualified t ty) v1 v2
+  | Vloc_info li ty v1 v2 :
+    val_related ty v1 v2 ->
+    val_related (TLocInfo li ty) v1 v2
   | Vraw_uint8 raw z (Hraw : raw_bytes_of_val σ Tbyte (Vint z) [raw]) :
     val_related Tbyte (Vraw raw) (Vint z)
   | Vuint8_raw z raw (Hraw : raw_bytes_of_val σ Tbyte (Vint z) [raw]) :
@@ -446,6 +449,10 @@ Module Type RAW_BYTES_MIXIN
     val_related (Tqualified q ty) v1 v2.
   Proof. by constructor. Qed.
 
+  Lemma val_related_loc_info {σ} li ty v1 v2 :
+    val_related (TLocInfo li ty) v1 v2 <-> val_related ty v1 v2.
+  Proof. split; first by inversion 1; subst; auto. by constructor. Qed.
+
   #[global] Instance val_related_equivalence {σ} ty : Equivalence (val_related ty).
   Proof.
     split; red.
@@ -453,6 +460,7 @@ Module Type RAW_BYTES_MIXIN
     { induction 1; auto. }
     intros v1 v2. induction 1.
     { done. }
+    { inversion 1; simplify_eq; auto. }
     { inversion 1; simplify_eq; auto. }
     { inversion 1; simplify_eq; auto.
       have [->] := raw_bytes_of_val_unique_encoding Hraw Hraw0. auto. }
@@ -641,6 +649,20 @@ Module Type HAS_TYPE_MIXIN (Import P : PTRS) (Import R : RAW_BYTES) (Import V : 
       has_type_prop (Vfloat f z) (Tfloat_ f).
     Proof. rewrite has_type_prop_float; eauto. Qed.
 
+    Lemma has_type_prop_drop_loc_info :
+      forall v ty, has_type_prop v ty <-> has_type_prop v (drop_loc_info ty).
+    Proof.
+      induction ty; cbn; try reflexivity.
+      { split; intro H.
+        - apply (proj1 (has_type_prop_qual_iff (drop_loc_info ty) q v)).
+          apply (proj1 IHty), (proj2 (has_type_prop_qual_iff ty q v)), H.
+        - apply (proj1 (has_type_prop_qual_iff ty q v)).
+          apply (proj2 IHty), (proj2 (has_type_prop_qual_iff (drop_loc_info ty) q v)), H. }
+      { split; intro H.
+        - apply (proj1 IHty), (proj1 (has_type_prop_loc_info v l ty)), H.
+        - apply (proj2 (has_type_prop_loc_info v l ty)), (proj2 IHty), H. }
+    Qed.
+
     Lemma has_type_prop_drop_qualifiers :
       forall v ty, has_type_prop v ty <-> has_type_prop v (drop_qualifiers ty).
     Proof.
@@ -725,5 +747,6 @@ Proof.
   induction 1.
   { done. }
   { by rewrite -!has_type_prop_qual_iff. }
+  { by rewrite !has_type_prop_loc_info. }
   all: by rewrite has_type_prop_raw_bytes_of_val.
 Qed.
